add heap camera for points-to predicates

IrisCore/BaseLogicShallow.thy
@@ -31,9 +31,12 @@ instance by (standard; auto simp: is_chain_def; transfer; auto)
   (meson le_refl ne_sprop_weaken ofe_refl total_n_inclI valid_raw_non_expansive)
 end
 
-lemma upred_f_ne: "\<lbrakk>n_equiv m P Q; m\<le>n; n_valid x m; Rep_upred_f Q x n\<rbrakk> \<Longrightarrow> Rep_upred_f Q x m"
+lemma upred_f_ne: "\<lbrakk>n_equiv m (P::('a::ucamera) upred_f) Q; m\<le>n; n_valid x m; Rep_upred_f Q x n\<rbrakk> 
+  \<Longrightarrow> Rep_upred_f Q x m"
   by (transfer; auto simp: n_incl_def) (metis \<epsilon>_left_id camera_comm ofe_refl) 
 
+
+text \<open> Basic predicates and predicate connectives: \<close>
 (* Arcane Isabelle magic, presented to you by Manuel Eberl *)
 context assumes "SORT_CONSTRAINT('a::ucamera)"
 begin
@@ -54,6 +57,9 @@ lemma upred_weaken: "\<lbrakk>n_equiv n x y; m\<le>n;upred_def f; f x n\<rbrakk>
 lemma upred_weaken_simple: "\<lbrakk>upred_def f; f x n; m\<le>n\<rbrakk> \<Longrightarrow> f x m"
   using ofe_refl upred_weaken by blast 
 
+lift_definition upred_f_holds :: "'a upred_f \<Rightarrow> bool" is
+  "\<lambda>u. \<forall>a n. n_valid a n \<longrightarrow>  u a n" .
+  
 (* This shows that upred_f are pointwise down-closes, non-expansive and monotone. *)
 theorem upred_equiv_upred_f: 
   "upred_def f \<longleftrightarrow> 
@@ -77,18 +83,18 @@ lemma upred_ne: "\<lbrakk>upred_def f; n_equiv n x y\<rbrakk> \<Longrightarrow> 
   
 text \<open> The semantic of uniform predicates is defined as a shallow embedding. \<close>
 
-lift_definition uPure :: "bool \<Rightarrow> 'a upred_f" ("\<upharpoonleft>_") is "\<lambda>b. \<lambda>_::'a. \<lambda>_::nat. b" .
+lift_definition upred_pure :: "bool \<Rightarrow> 'a upred_f" ("\<upharpoonleft>_") is "\<lambda>b::bool. \<lambda>_::'a. \<lambda>_::nat. b" .
 
-lift_definition upred_eq :: "'b::ofe \<Rightarrow> 'b \<Rightarrow> 'a upred_f" (infix "=\<^sub>u" 60) is 
-  "\<lambda>x (y::'b). \<lambda>_::'a. \<lambda>n. ofe_class.n_equiv n x y" by (rule ofe_mono)
+lift_definition upred_eq :: "'c::ofe \<Rightarrow> 'c \<Rightarrow> 'a upred_f" (infix "=\<^sub>u" 60) is 
+  "\<lambda>x (y::'c). \<lambda>_::'a. \<lambda>n. ofe_class.n_equiv n x y" by (rule ofe_mono)
 
 lift_definition upred_conj :: "'a upred_f \<Rightarrow> 'a upred_f \<Rightarrow> 'a upred_f" (infixl "\<and>\<^sub>u" 60) is
-  "\<lambda>x y a n. x a n \<and> y a n" by (rule conj_forward)
+  "\<lambda>P Q (a::'a) (n::nat). P a n \<and> Q a n" by (rule conj_forward)
 lift_definition upred_disj :: "'a upred_f \<Rightarrow> 'a upred_f \<Rightarrow> 'a upred_f" (infixl "\<or>\<^sub>u" 60) is
-  "\<lambda>x y a n. x a n \<or> y a n" by (rule disj_forward)
+  "\<lambda>P Q (a::'a) (n::nat). P a n \<or> Q a n" by (rule disj_forward)
 
 lift_definition upred_impl :: "'a upred_f \<Rightarrow> 'a upred_f \<Rightarrow> 'a upred_f" (infixr "\<longrightarrow>\<^sub>u" 60) is
-  "\<lambda>x y (a::'a) n. (\<forall>m\<le>n. \<forall>b. incl a b \<longrightarrow> n_valid b m \<longrightarrow> x b m \<longrightarrow> y b m)"
+  "\<lambda>P Q (a::'a) n. (\<forall>m\<le>n. \<forall>b. incl a b \<longrightarrow> n_valid b m \<longrightarrow> P b m \<longrightarrow> Q b m)"
 proof -
   fix x y n n' a b m c
   assume assms: "n_incl n' a (b::'a)" "n'\<le>n" "m\<le>n'" "incl b c" "n_valid c m" "x c m" 
@@ -113,14 +119,14 @@ proof -
   show "y c m".
 qed
 
-lift_definition upred_forall :: "('b \<Rightarrow> 'a upred_f) \<Rightarrow> 'a upred_f" ("\<forall>\<^sub>u _") is "\<lambda>f a n. \<forall>x. f x a n" 
-  by (rule meta_allE)
+lift_definition upred_forall :: "('c \<Rightarrow> 'a upred_f) \<Rightarrow> 'a upred_f" ("\<forall>\<^sub>u _") is 
+  "\<lambda>P (a::'a) (n::nat). \<forall>x::'c. P x a n" by (rule meta_allE)
 
-lift_definition upred_exists :: "('b \<Rightarrow> 'a upred_f) \<Rightarrow> 'a upred_f" ("\<exists>\<^sub>u _") is "\<lambda>f a n. \<exists>x. f x a n"
-  by (rule ex_forward)
+lift_definition upred_exists :: "('c \<Rightarrow> 'a upred_f) \<Rightarrow> 'a upred_f" ("\<exists>\<^sub>u _") is 
+  "\<lambda>P (a::'a) (n::nat). \<exists>x::'c. P x a n" by (rule ex_forward)
 
 lift_definition upred_sep :: "'a upred_f \<Rightarrow> 'a upred_f \<Rightarrow> 'a upred_f" (infixl "\<^emph>" 80) is
-  "\<lambda>x y a n. \<exists>b1 b2. n_equiv n a (op b1 b2) \<and> x b1 n \<and> y b2 n"
+  "\<lambda>P Q (a::'a) n. \<exists>b1 b2. n_equiv n a (b1 \<cdot> b2) \<and> P b1 n \<and> Q b2 n"
 proof auto
   fix P Q n m a b c1 c2
   assume assms: "n_incl m a (b::'a)" "m\<le>n"
@@ -138,7 +144,7 @@ proof auto
 qed
 
 lift_definition upred_wand :: "'a upred_f \<Rightarrow> 'a upred_f \<Rightarrow> 'a upred_f" (infixr "-\<^emph>" 60) is 
-  "\<lambda>P Q a n. \<forall>b m. m\<le>n \<longrightarrow> n_valid (op a b) m \<longrightarrow> P b m \<longrightarrow> Q (op a b) m"
+  "\<lambda>P Q (a::'a) n. \<forall>b m. m\<le>n \<longrightarrow> n_valid (a \<cdot> b) m \<longrightarrow> P b m \<longrightarrow> Q (a \<cdot> b) m"
 proof -
   fix P Q n n' a b c m
   assume Q: "\<And>n m x y. Q (x::'a) n \<Longrightarrow> n_incl m x y \<Longrightarrow> m \<le> n \<Longrightarrow> Q y m"
@@ -149,13 +155,13 @@ proof -
   show "Q (op b c) m" .
 qed
 
-lift_definition upred_own :: "'a \<Rightarrow> 'a upred_f" ("Own(_)") is "\<lambda>a b n. n_incl n a b" 
+lift_definition upred_own :: "'a \<Rightarrow> 'a upred_f" ("Own(_)") is "\<lambda>(a::'a) b n. n_incl n a b" 
 unfolding n_incl_def using camera_assoc op_equiv_subst by metis
 
-lift_definition upred_valid :: "'a \<Rightarrow> 'a upred_f" ("\<V>(_)") is "\<lambda>a _. n_valid a" 
+lift_definition upred_valid :: "'b::camera \<Rightarrow> 'a upred_f" ("\<V>(_)") is "\<lambda>(a::'b) (_::'a). n_valid a" 
   using Rep_sprop n_incl_def by blast
   
-lift_definition upred_persis :: "'a upred_f \<Rightarrow> 'a upred_f" ("\<box>_") is "\<lambda>P a. P (core a)"
+lift_definition upred_persis :: "'a upred_f \<Rightarrow> 'a upred_f" ("\<box>_") is "\<lambda>P (a::'a) n. (P (core a) n)::bool"
 proof (auto simp: n_incl_def)
   fix f n m 
   fix a b c :: 'a
@@ -167,30 +173,106 @@ proof (auto simp: n_incl_def)
   from I[OF assms(1) this assms(2)] show "f (core b) m" .
 qed
 
-lift_definition upred_plain :: "'a upred_f \<Rightarrow> 'a upred_f" ("\<^item>_") is "\<lambda>P _ n. P \<epsilon> n"
+lift_definition upred_plain :: "'a upred_f \<Rightarrow> 'a upred_f" ("\<^item>_") is "\<lambda>P (_::'a) (n::nat). (P (\<epsilon>::'a) n)::bool"
   by (metis \<epsilon>_left_id ofe_eq_limit n_incl_def)
 
-lift_definition upred_later :: "'a upred_f \<Rightarrow> 'a upred_f" ("\<triangleright>_") is "\<lambda>P a n. n=0 \<or> P a (n-1)" 
+lift_definition upred_later :: "'a upred_f \<Rightarrow> 'a upred_f" ("\<triangleright>_") is "\<lambda>P (a::'a) n. n=0 \<or> P a (n-1)" 
   by (smt (verit, ccfv_SIG) n_incl_def diff_0_eq_0 diff_diff_cancel diff_is_0_eq diff_right_commute diff_self_eq_0 ofe_mono)
 
 lift_definition upred_bupd :: "'a upred_f \<Rightarrow> 'a upred_f" ("\<Rrightarrow>_") is
-  "\<lambda>P a n. \<forall>m b. m\<le>n \<longrightarrow> n_valid (op a b) m \<longrightarrow> (\<exists>c. n_valid (op c b) m \<and> P c m)"
+  "\<lambda>P (a::'a) n. \<forall>m b. m\<le>n \<longrightarrow> n_valid (a \<cdot> b) m \<longrightarrow> (\<exists>c. n_valid (c \<cdot> b) m \<and> P c m)"
   by (meson dual_order.trans n_incl_def n_valid_incl_subst)
 
 lift_definition upred_entails :: "'a upred_f \<Rightarrow> 'a upred_f \<Rightarrow> bool" (infix "\<turnstile>" 50) is
-  "\<lambda>P Q. \<forall>a n. n_valid a n \<longrightarrow> P a n \<longrightarrow> Q a n" .
+  "\<lambda>P Q. \<forall>(a::'a) n. n_valid a n \<longrightarrow> P a n \<longrightarrow> Q a n" .
 
 definition upred_entail_eq :: "'a upred_f \<Rightarrow> 'a upred_f \<Rightarrow> bool" (infix "\<stileturn>\<turnstile>" 40) where
   "P \<stileturn>\<turnstile> Q \<equiv> (upred_entails P Q) \<and> (upred_entails Q P)"
 end
 
+text \<open> Basic properties of upred predicates: \<close>
+
 lemma upred_entail_eq_simp: "P\<stileturn>\<turnstile>Q \<equiv> \<forall>a n. n_valid a n \<longrightarrow> Rep_upred_f P a n = Rep_upred_f Q a n"
-  by (auto simp: upred_entail_eq_def upred_entails.rep_eq) (smt (verit))
+  by (auto simp: upred_entail_eq_def upred_entails.rep_eq) (smt (verit, best))
 lemma upred_entail_eqE: "P\<stileturn>\<turnstile>Q \<Longrightarrow> (\<And>a n. n_valid a n \<Longrightarrow> Rep_upred_f P a n = Rep_upred_f Q a n)"
-  using upred_entail_eq_simp by auto  
+  using upred_entail_eq_simp by auto
 lemma upred_entail_eqI: "(\<And>a n. n_valid a n \<Longrightarrow> Rep_upred_f P a n = Rep_upred_f Q a n) \<Longrightarrow> P\<stileturn>\<turnstile>Q"
   using upred_entail_eq_simp by auto
+
+lemma upred_entail_eqL: "P\<stileturn>\<turnstile>Q \<Longrightarrow> P\<turnstile>Q" by (simp add: upred_entail_eq_def)
+lemma upred_entail_eqR: "P\<stileturn>\<turnstile>Q \<Longrightarrow> Q\<turnstile>P" by (simp add: upred_entail_eq_def)
+
+lemma upred_entails_trans: "\<lbrakk>P\<turnstile>Q; Q\<turnstile>R\<rbrakk> \<Longrightarrow> P\<turnstile>R"
+  by (auto simp: upred_entails.rep_eq)
+
+lemma own_valid: "Own(a) \<turnstile> \<V>(a)"
+  apply (auto simp: upred_entails.rep_eq upred_own.rep_eq upred_valid.rep_eq n_incl_def)
+  using camera_valid_op n_valid_ne by blast
+
+lemma upred_holds_entails: "upred_f_holds P \<longleftrightarrow> ((\<upharpoonleft>True) \<turnstile> P)"
+  by (auto simp: upred_f_holds.rep_eq upred_entails.rep_eq upred_pure.rep_eq)
+
+lemma upred_entailsE: "P \<turnstile> Q \<Longrightarrow> (\<And>a n. \<lbrakk>n_valid a n; Rep_upred_f P a n\<rbrakk> \<Longrightarrow> Rep_upred_f Q a n)"
+  by (auto simp: upred_entails.rep_eq)
+
+lemma upred_wandI: "(P \<^emph> Q) \<turnstile> R \<Longrightarrow> P \<turnstile> (Q-\<^emph>R)"
+  apply (auto simp: upred_entails.rep_eq upred_sep.rep_eq upred_wand.rep_eq)
+  using ofe_refl upred_def_rep upred_weaken_simple by blast
+
+lemma upred_true_sep: "(P \<^emph> \<upharpoonleft>True) = P"
+  apply transfer using n_incl_def by fastforce
+
+lemma upred_sep_comm: "P \<^emph> Q = Q \<^emph> P"
+  by transfer (metis (no_types, opaque_lifting) camera_comm)
+
+lemma upred_wand_holdsI: "Q \<turnstile> R \<Longrightarrow> upred_f_holds (Q-\<^emph>R)"
+  by (metis upred_wandI upred_holds_entails upred_true_sep upred_sep_comm)
+
+lemma upred_own_core_persis: "Own(a) \<turnstile> \<box>Own(core a)"
+  by (auto simp: upred_entails.rep_eq upred_own.rep_eq upred_persis.rep_eq camera_core_mono_n)
+
+lemma upred_entails_wand_holdsL: "\<lbrakk>P \<turnstile> Q; upred_f_holds (Q-\<^emph>R)\<rbrakk> \<Longrightarrow> upred_f_holds (P-\<^emph>R)"
+  by transfer (metis camera_comm camera_valid_op)
+
+lemma upred_entails_wand_holdsR: "\<lbrakk>Q \<turnstile> R; upred_f_holds (P-\<^emph>Q)\<rbrakk> \<Longrightarrow> upred_f_holds (P-\<^emph>R)"
+  by transfer auto
+
+lemma upred_entails_wand_holdsR2: "\<lbrakk>Q \<turnstile> R; upred_f_holds (P1-\<^emph>P2-\<^emph>Q)\<rbrakk> \<Longrightarrow> upred_f_holds (P1-\<^emph>P2-\<^emph>R)"
+  by transfer auto
+
+lemma pure_entailsI: "(p \<Longrightarrow> q) \<Longrightarrow> \<upharpoonleft>p\<turnstile>\<upharpoonleft>q"
+  by (auto simp: upred_pure_def upred_entails.rep_eq Abs_upred_f_inverse)
   
+lemma discrete_valid: "\<V>(a::'a::dcamera) \<stileturn>\<turnstile> \<upharpoonleft>(valid a)"
+  apply (rule upred_entail_eqI; auto simp: upred_valid.rep_eq upred_pure.rep_eq)
+  using dcamera_valid_iff by blast+
+
+lemma own_op: "Own(a\<cdot>b) \<stileturn>\<turnstile> Own(a) \<^emph> Own(b)"
+  apply (rule upred_entail_eqI)
+  apply (auto simp: upred_own.rep_eq upred_sep.rep_eq)
+  apply (metis camera_assoc n_incl_def n_incl_op_extend n_incl_refl)
+  by (smt (z3) camera_assoc camera_comm n_incl_def ofe_trans op_equiv)
+
+lemma own_valid2: "upred_f_holds (Own(a1) -\<^emph> Own (a2) -\<^emph> \<V>(a1\<cdot>a2))"
+  apply (rule upred_wand_holdsI)
+  apply (rule upred_wandI)
+  using own_op own_valid upred_entails_trans upred_entail_eq_def by blast
+
 (* Simple definition of iprop due to the axiomatic character of our work. *)
 type_synonym 'a iprop = "'a upred_f"
+
+text \<open> Persistent predicates \<close>
+definition persistent :: "('a::ucamera) iprop \<Rightarrow> bool" where "persistent P \<equiv> P \<turnstile> \<box>P"
+
+lemma persistent_persis: "persistent (\<box>P)"
+  by (auto simp: persistent_def upred_persis.rep_eq upred_entails.rep_eq camera_core_idem)
+
+lemma persistent_pure: "persistent (\<upharpoonleft>P)"
+  by (auto simp: persistent_def upred_persis.rep_eq upred_entails.rep_eq upred_pure.rep_eq)  
+
+lemma persistent_valid: "persistent (\<V>(a))"
+  by (auto simp: persistent_def upred_persis.rep_eq upred_entails.rep_eq upred_valid.rep_eq)
+
+lemma persistent_core_own: "persistent (Own(a::'a::{core_id,ucamera}))"
+  by (auto simp: persistent_def upred_persis.rep_eq upred_entails.rep_eq upred_own.rep_eq core_id)  
 end
