IrisCore/PointTo.thy
@@ -25,16 +25,14 @@ begin
 
   Functions:
 
-  points_to :: "loc \<Rightarrow> dfrac \<Rightarrow> val \<Rightarrow> \<Sigma> iProp" where "points_to l dq v = mapsto l dg (Some v)"
-  mapsto :: "'loc \<Rightarrow> dfrac \<Rightarrow> 'val \<Rightarrow> \<Sigma> iProp" where "mapsto l dq v = ghost_map_elem gen_heap_name l dq v"
-  ghost_map_elem :: "gname \<Rightarrow> 'key \<Rightarrow> dfrac \<Rightarrow> 'val \<Rightarrow> \<Sigma> iProp" where 
-    "ghost_map_elem \<gamma> k dq v = Own_\<gamma>(gmap_view_frag k dq v)"
-  gmap_view_frag :: "'key \<Rightarrow> dfrac \<Rightarrow> 'val \<Rightarrow> ('key,'val) gmap_view" where
+  fun points_to :: "loc \<Rightarrow> dfrac \<Rightarrow> val \<Rightarrow> \<Sigma> iProp" where "points_to l dq v = mapsto l dg (Some v)"
+  fun mapsto :: "'loc \<Rightarrow> dfrac \<Rightarrow> 'val \<Rightarrow> \<Sigma> iProp" where 
+    "mapsto l dq v = ghost_map_elem gen_heap_name l dq v"
+  fun ghost_map_elem :: "gname \<Rightarrow> 'key \<Rightarrow> dfrac \<Rightarrow> 'val \<Rightarrow> \<Sigma> iProp" where 
+    "ghost_map_elem \<gamma> k dq v = Own_\<gamma>(gmap_view_frag k dq v)" <----------------- This is problematic!
+  fun gmap_view_frag :: "'key \<Rightarrow> dfrac \<Rightarrow> 'val \<Rightarrow> ('key,'val) gmap_view" where
     "gmap_view_frag k dq v = view_frag [k\<mapsto>(dq,Abs_ag v)]"
-  view_frag :: "'b \<Rightarrow> ('a,'b) view" where "view_frag b = View None b"
-
-  ported points_to :: "loc \<Rightarrow> dfrac \<Rightarrow> val \<Rightarrow> iProp" where
-    "points_to l dq v = Own([k\<mapsto>(dq, Abs_ag (Some v))])"
+  fun view_frag :: "'b \<Rightarrow> ('a,'b) view" where "view_frag b = View None b"
   
   Types:
 
@@ -42,8 +40,7 @@ begin
   datatype ('a,'b) view = View (view_auth_proj: "(dfrac\<times>'a ag) option") (view_frag_proj: 'b)
 
   NOTE: view is a dependent type that has a relation function between 'a and 'b.
-  This can be more or less ported to being a type class, I think?!!?!?!
-
+  This can be more or less ported to being a type class, I think?
 
   PROBLEM!!!! 
   The way that meta data is included in the gen_heap can not simply be transferred to Isabelle.
@@ -56,9 +53,245 @@ begin
   data but it is a real big issue for a complete port to Isabelle!
 *)
 
-type_synonym ('l,'v) heap = "'l \<rightharpoonup> (dfrac\<times>'v ag)"
+text \<open> An own heap camera that is a simplification of the one used in the Coq implementation. \<close>
+datatype ('l,'v::ofe) heap = Heap "'l \<rightharpoonup> (dfrac\<times>'v ag)"
 
-definition points_to :: "'l \<Rightarrow> dfrac \<Rightarrow> 'v::ofe \<Rightarrow> ('l,'v option) heap iprop" where
-  "points_to l dq v = Own([l\<mapsto>(dq, Abs_ag {Some v})])"
+instantiation heap :: (type, ofe) ofe begin
+fun n_equiv_heap :: "nat \<Rightarrow> ('a, 'b) heap \<Rightarrow> ('a, 'b) heap \<Rightarrow> bool" where
+  "n_equiv_heap n (Heap x) (Heap y) = n_equiv n x y"
+fun ofe_eq_heap :: "('a, 'b) heap \<Rightarrow> ('a, 'b) heap \<Rightarrow> bool" where
+  "ofe_eq_heap (Heap x) (Heap y) = ofe_eq x y"
+instance proof
+  show "\<And>n (x::('a, 'b) heap). n_equiv n x x" by (cases rule: heap.induct) (auto simp: ofe_refl)
+next
+  fix x y :: "('a, 'b) heap" fix n
+  show "n_equiv n x y = n_equiv n y x" by (cases x; cases y) (auto simp: ofe_sym)
+next
+  fix x y z :: "('a, 'b) heap" fix n
+  show "n_equiv n x y \<Longrightarrow> n_equiv n y z \<Longrightarrow> n_equiv n x z"
+    by (cases x; cases y; cases z) (auto intro: ofe_trans)
+next
+  fix x y :: "('a, 'b) heap" fix n m
+  show "m \<le> n \<Longrightarrow> n_equiv n x y \<Longrightarrow> n_equiv m x y" by (cases x; cases y) (auto simp: ofe_mono)
+next
+  fix x y :: "('a, 'b) heap"
+  show "ofe_eq x y = (\<forall>n. n_equiv n x y)" by (cases x; cases y) (auto simp: ofe_limit)
+next
+  fix x y :: "('a, 'b) heap"
+  show "x = y \<Longrightarrow> ofe_eq x y" by (cases x; cases y) (auto simp: ofe_eq_eq)
+qed
+end
+instance heap :: (type, discrete) discrete
+proof
+  fix a b :: "('a, 'b) heap" fix n
+  show "n_equiv n a b = (a = b)" by (cases a; cases b) (auto simp: d_equiv)
+next
+  fix a b :: "('a, 'b) heap"
+  show "ofe_eq a b = (a = b)" by (cases a; cases b) (auto simp: d_eq)
+qed
 
+abbreviation "heap_rel \<equiv> \<lambda>m n.
+  \<forall>l a b. Some(a,b) = (m::'l \<rightharpoonup> (dfrac\<times>'v::ofe ag)) l \<longrightarrow> (valid a \<and> (\<exists>ag. n_equiv n b (to_ag ag)))"
+
+lemma heap_valid: "heap_rel m n \<Longrightarrow> n_valid m n"
+  apply (auto simp: valid_raw_fun.rep_eq valid_raw_option_def valid_raw_prod_def sprop_conj.rep_eq split: option.splits)
+  apply (metis valid_dfrac)
+  by (metis n_valid_ne ofe_sym to_ag.rep_eq valid_raw_ag.rep_eq)
+
+lemma heap_rel_mono: "\<lbrakk>heap_rel m1 n; n_incl m m2 m1; m\<le>n\<rbrakk> \<Longrightarrow> heap_rel m2 m"
+proof (auto simp: n_incl_def)
+  fix a b c l
+  assume assms: "heap_rel m1 n" "m\<le>n" "n_equiv m m1 (m2\<cdot>c)" "Some (a,b) = m2 l" 
+  then have "\<forall>i. n_equiv m (m1 i) ((m2 i) \<cdot> (c i))" by (simp add: n_equiv_fun_def op_fun_def)
+  with assms(4) have equiv: "n_equiv m (m1 l) ((Some (a,b)) \<cdot> (c l))" by simp
+  moreover obtain a2 b2 where ab2: "Some (a2,b2) = (Some (a,b)) \<cdot> (c l)" by (auto simp: op_option_def)
+    (metis option_op.elims surj_pair)
+  ultimately obtain a1 b1 where ab1: "Some (a1,b1) = m1 l" by (auto simp: n_equiv_option_def)
+  from ab1 assms(1) have "valid a1" by simp
+  from equiv ab1 ab2 have "n_equiv m a1 a2" by (auto simp: n_equiv_option_def)
+  with \<open>valid a1\<close> have "valid a2" by simp
+  show "valid a" proof (cases "c l")
+    case None
+    with ab2 have "a2 = a" by (simp add: op_option_def)
+    with \<open>valid a2\<close> show ?thesis by simp
+  next
+    case (Some cl)
+    then obtain ac bc where abc: "cl = (ac,bc)" by fastforce
+    with Some ab2 have "a2 = a \<cdot> ac" by (simp add: op_option_def op_prod_def)
+    with \<open>valid a2\<close> show ?thesis using camera_valid_op valid_dfrac by blast
+  qed
+next
+  fix a b c l
+  assume assms: "heap_rel m1 n" "m\<le>n" "n_equiv m m1 (m2\<cdot>c)" "Some (a,b) = m2 l" 
+  then have "\<forall>i. n_equiv m (m1 i) ((m2 i) \<cdot> (c i))" by (simp add: n_equiv_fun_def op_fun_def)
+  with assms(4) have equiv: "n_equiv m (m1 l) ((Some (a,b)) \<cdot> (c l))" by simp
+  moreover obtain a2 b2 where ab2: "Some (a2,b2) = (Some (a,b)) \<cdot> (c l)" by (auto simp: op_option_def)
+    (metis option_op.elims surj_pair)
+  ultimately obtain a1 b1 where ab1: "Some (a1,b1) = m1 l" by (auto simp: n_equiv_option_def)
+  from assms(1) ab1 obtain ag1 where ag1: "n_equiv m b1 (to_ag ag1)" using assms(2) ofe_mono by blast
+  from equiv ab1 ab2 have "n_equiv m b1 b2" by (auto simp: n_equiv_option_def)
+  with ag1 have ag2:"n_equiv m b2 (to_ag ag1)" using ofe_trans ofe_sym by blast
+  show "\<exists>ag. n_equiv m b (to_ag ag)" proof (cases "c l")
+    case None
+    with ab2 have "b2=b" by (simp add: op_option_def)
+    with ag2 show ?thesis by auto
+  next
+    case (Some cl)
+    then obtain ac bc where abc: "cl = (ac,bc)" by fastforce
+    with Some ab2 have "b2 = b \<cdot> bc" by (simp add: op_option_def op_prod_def)
+    with ag2 have ag_equiv: "n_equiv m (to_ag ag1) (b\<cdot>bc)" by (simp add: ofe_sym)
+    from to_ag_valid have "n_valid (to_ag ag1) m" by (auto simp: valid_def)
+    from camera_extend[OF this ag_equiv] obtain c1 c2 where cag:
+      "to_ag ag1 = c1 \<cdot> c2 \<and> n_equiv m c1 b \<and> n_equiv m c2 bc" by auto
+    with to_ag_op have "c1 = to_ag ag1" "c2 = to_ag ag1" by blast+
+    with cag show ?thesis by (auto simp: ofe_sym)
+  qed
+qed
+  
+instantiation heap :: (type, ofe) camera begin
+lift_definition valid_raw_heap :: "('a, 'b) heap \<Rightarrow> sprop" is
+  "\<lambda>x n. case x of Heap m \<Rightarrow> heap_rel m n"
+  apply (auto split: heap.splits) using ofe_refl ofe_mono by blast
+definition pcore_heap :: "('a, 'b) heap \<Rightarrow> ('a, 'b) heap option" where
+  "pcore_heap x = (case x of Heap x \<Rightarrow> Some (Heap (core x)))"
+fun op_heap :: "('a, 'b) heap \<Rightarrow> ('a, 'b) heap \<Rightarrow> ('a, 'b) heap" where
+  "op_heap (Heap x) (Heap y) = Heap (x \<cdot> y)"
+instance proof
+show "non_expansive (valid_raw::('a, 'b) heap \<Rightarrow> sprop)" proof (rule non_expansiveI)
+  fix x y :: "('a,'b) heap" fix n
+  assume assm: "n_equiv n x y"
+  then obtain xm ym where m: "x=Heap xm" "y=Heap ym" by (rule n_equiv_heap.elims) simp
+  with assm have "n_equiv n xm ym" by simp
+  then have l_equiv: "\<forall>l. n_equiv n (xm l) (ym l)" by (auto simp: n_equiv_fun_def)
+  then have xy_val: "\<forall>a b. Some (a, b) = xm l \<longrightarrow> valid a \<Longrightarrow> \<forall>c d. Some (c, d) = ym l \<longrightarrow> valid c" for l
+    by (smt (verit, ccfv_SIG) Pair_inject n_equiv_option_def n_equiv_prod.elims(2) n_valid_ne option.sel valid_dfrac)
+  have xy_ag: "m\<le>n \<Longrightarrow> \<forall>l a b. Some (a, b) = xm l \<longrightarrow> valid a \<and> (\<exists>ag. n_equiv m b (to_ag ag)) 
+    \<Longrightarrow> Some (c, d) = ym l \<longrightarrow> (\<exists>ag. n_equiv m d (to_ag ag))" for l c d m
+    by (smt (verit, ccfv_threshold) l_equiv n_equiv_option_def n_equiv_prod.elims(2) ofe_mono ofe_sym ofe_trans old.prod.inject option.inject)
+  from l_equiv have yx_val: "\<forall>a b. Some (a, b) = ym l \<longrightarrow> valid a \<Longrightarrow> \<forall>c d. Some (c, d) = xm l \<longrightarrow> valid c" for l
+    by (smt (verit, ccfv_SIG) Pair_inject d_equiv n_equiv_option_def n_equiv_prod.elims(2) option.inject)
+  have yx_ag: "m\<le>n \<Longrightarrow> \<forall>a b. Some (a, b) = ym l \<longrightarrow> (\<exists>ag. n_equiv m b (to_ag ag)) 
+    \<Longrightarrow> Some (c, d) = xm l \<longrightarrow> (\<exists>ag. n_equiv m d (to_ag ag))" for c d l m
+    by (smt (verit, ccfv_SIG) Pair_inject l_equiv n_equiv_option_def n_equiv_prod.elims(2) ofe_mono ofe_trans option.sel)
+  show "n_equiv n (valid_raw x) (valid_raw y)"
+    apply (auto simp: valid_raw_heap.rep_eq n_equiv_sprop_def split: heap.splits)
+    using m xy_val xy_ag yx_val yx_ag apply blast+
+    using m yx_ag by blast
+  qed
+next    
+show "non_expansive (pcore::('a, 'b) heap \<Rightarrow> ('a, 'b) heap option)" by (rule non_expansiveI)
+  (auto simp: pcore_heap_def n_equiv_option_def core_ne[unfolded non_expansive_def] split: heap.splits)
+next
+show " non_expansive2 (op::('a, 'b) heap \<Rightarrow> ('a, 'b) heap \<Rightarrow> ('a, 'b) heap)" by (rule non_expansive2I)
+  (smt (verit, best) heap.inject n_equiv_heap.elims(2) n_equiv_heap.elims(3) op_heap.simps op_ne)
+next
+fix a b c :: "('a, 'b) heap"
+show "a \<cdot> b \<cdot> c = a \<cdot> (b \<cdot> c)" by (cases a; cases b; cases c) (auto simp: camera_assoc)
+next
+fix a b :: "('a, 'b) heap"
+show "a \<cdot> b = b \<cdot> a" by (cases a; cases b) (auto simp: camera_comm)
+next
+fix a a' :: "('a, 'b) heap"
+show "pcore a = Some a' \<Longrightarrow> a' \<cdot> a = a" by (cases a; cases a') 
+  (auto simp: pcore_heap_def camera_core_id)
+next
+fix a a' :: "('a, 'b) heap"
+show "pcore a = Some a' \<Longrightarrow> pcore a' = pcore a" 
+  by (cases a; cases a') (auto simp: pcore_heap_def camera_core_idem)
+next
+fix a a' b :: "('a, 'b) heap"
+show "pcore a = Some a' \<Longrightarrow> \<exists>c. b = a \<cdot> c \<Longrightarrow> \<exists>b'. pcore b = Some b' \<and> (\<exists>c. b' = a' \<cdot> c)"
+  apply (cases a; cases a'; cases b) apply (auto simp: pcore_heap_def)
+  using camera_core_mono[unfolded incl_def] heap.inject
+  by (metis (no_types, opaque_lifting) PointTo.op_heap.elims PointTo.op_heap.simps)
+next
+fix a b :: "('a, 'b) heap" fix n
+show "Rep_sprop (valid_raw (a \<cdot> b)) n \<Longrightarrow> Rep_sprop (valid_raw a) n"
+  proof (cases a; cases b; simp add: valid_raw_heap.rep_eq)
+  fix x y
+  assume assms: "heap_rel (x\<cdot>y) n" "a=Heap x" "b=Heap y"
+  from heap_rel_mono[OF assms(1), of n x] show "heap_rel x n"  by (simp add: n_incl_op_extend)
+  qed
+next
+fix a b c :: "('a, 'b) heap" fix n
+show "Rep_sprop (valid_raw a) n \<Longrightarrow> n_equiv n a (b \<cdot> c)
+  \<Longrightarrow> \<exists>c1 c2. a = c1 \<cdot> c2 \<and> n_equiv n c1 b \<and> n_equiv n c2 c"
+  proof (cases a; cases b; cases c ; auto simp: valid_raw_heap.rep_eq)
+  fix x y z
+  assume assms: "\<forall>l a b. Some (a, b) = x l \<longrightarrow>camera_class.valid a \<and> (\<exists>ag. n_equiv n b (to_ag ag))" 
+  "n_equiv n x (y \<cdot> z)" "a = Heap x" "b = Heap y" "c = Heap z"
+  from heap_valid[OF assms(1)] have "n_valid x n" .
+  from camera_extend[OF this assms(2)] have "\<exists>c1 c2. x = c1 \<cdot> c2 \<and> n_equiv n c1 y \<and> n_equiv n c2 z" .
+  then show "\<exists>c1 c2. Heap x = c1 \<cdot> c2 \<and> n_equiv n c1 (Heap y) \<and> n_equiv n c2 (Heap z)"
+    by (metis n_equiv_heap.simps op_heap.simps)
+  qed
+qed
+end
+
+instance heap :: (type, discrete) dcamera by standard 
+  (auto simp: valid_raw_heap.rep_eq valid_def d_equiv split: heap.splits)
+
+instantiation heap :: (type, ofe) ucamera begin
+  definition \<epsilon>_heap :: "('a, 'b) heap" where "\<epsilon>_heap \<equiv> Heap \<epsilon>"
+instance proof 
+  fix a :: "('a,'b) heap" 
+  have "Map.empty = \<epsilon>" by simp
+  with \<epsilon>_left_id have "Map.empty \<cdot> (x::('a \<rightharpoonup> (dfrac\<times>'b option ag))) = x" for x by (smt (verit))
+  then show "\<epsilon>\<cdot>a = a" by (cases a; auto simp: \<epsilon>_heap_def) (metis \<epsilon>_left_id \<open>Map.empty = \<epsilon>\<close>)
+next
+  have "Map.empty = \<epsilon>" by simp  
+  show "pcore \<epsilon> = Some (\<epsilon>::('a,'b) heap)" by (auto simp: pcore_heap_def \<epsilon>_heap_def)
+    (metis \<epsilon>_core \<open>Map.empty = \<epsilon>\<close>)
+qed (auto simp: \<epsilon>_heap_def valid_raw_heap.rep_eq valid_def split: heap.splits)
+end
+
+definition points_to :: "'l \<Rightarrow> dfrac \<Rightarrow> 'v::ofe \<Rightarrow> ('l,'v option) heap iprop" ("_ \<mapsto>{_} _" 60) where
+  "points_to l dq v = Own(Heap [l\<mapsto>(dq, to_ag (Some v))])"
+abbreviation points_to_disc :: "'l \<Rightarrow> 'v::ofe \<Rightarrow> ('l,'v option) heap iprop" (infix "\<mapsto>\<box>" 60) where 
+  "points_to_disc \<equiv> \<lambda>l v. (l \<mapsto>{DfracDiscarded} v)"
+abbreviation points_to_own :: "'l \<Rightarrow> frac \<Rightarrow> 'v::ofe \<Rightarrow> ('l,'v option) heap iprop" ("_\<mapsto>{#_}_" 60) where
+  "points_to_own \<equiv> \<lambda>l p v. (l\<mapsto>{DfracOwn p} v)"  
+abbreviation points_to_full :: "'l \<Rightarrow> 'v::ofe \<Rightarrow> ('l,'v option) heap iprop" (infix "\<mapsto>\<^sub>u" 60) where
+  "points_to_full \<equiv> \<lambda>l v. (l \<mapsto>{DfracOwn 1} v)"
+  
+lemma frag_map_valid: "valid (Heap [k\<mapsto>(dq,to_ag v)]) \<longleftrightarrow> valid dq"
+  apply (auto simp: valid_def valid_raw_heap.rep_eq)  using ofe_refl by blast
+
+lemma points_to_valid: "upred_f_holds ((l \<mapsto>{dq} (v::'v::discrete)) -\<^emph> \<upharpoonleft>(valid dq))"
+proof -
+  have "(l \<mapsto>{dq} v) \<turnstile> \<V>(Heap [l\<mapsto>(dq,to_ag (Some v))])" by (auto simp: points_to_def own_valid)
+  moreover have "\<V>(Heap [l\<mapsto>(dq,to_ag (Some v))]) \<turnstile> \<upharpoonleft>(valid(Heap [l\<mapsto>(dq,to_ag (Some v))]))"
+    using discrete_valid[of "Heap [l\<mapsto>(dq,to_ag (Some v))]"] upred_entail_eq_def by auto
+  ultimately have "(l \<mapsto>{dq} v) \<turnstile> \<upharpoonleft>(valid dq)" 
+    by (auto simp: frag_map_valid intro: upred_entails_trans)
+  from upred_wand_holdsI [OF this] show ?thesis .
+qed
+
+lemma map_op: "[l\<mapsto>(dq1, to_ag (Some v1))]\<cdot>[l\<mapsto>(dq2, to_ag (Some v2))] = 
+  [l\<mapsto>(dq1, to_ag (Some v1))\<cdot>(dq2, to_ag (Some v2))]"
+  by (auto simp: op_fun_def op_option_def)
+  
+lemma mapsto_agree: "upred_f_holds ((l \<mapsto>{dq1} (v1::'a::discrete)) -\<^emph> (l \<mapsto>{dq2} v2) -\<^emph> \<upharpoonleft>(v1 = v2))"
+proof -
+  have "upred_f_holds ((l \<mapsto>{dq1} v1) -\<^emph> (l \<mapsto>{dq2} v2) -\<^emph> 
+    \<V>(Heap [l\<mapsto>(dq1, to_ag (Some v1))]\<cdot>Heap [l\<mapsto>(dq2, to_ag (Some v2))]))"
+    apply (auto simp: points_to_def) using own_valid2 by (metis (no_types, lifting) op_heap.simps)
+  then have "upred_f_holds ((l \<mapsto>{dq1} v1) -\<^emph> (l \<mapsto>{dq2} v2) -\<^emph> 
+    \<V>(Heap ([l\<mapsto>(dq1, to_ag (Some v1))\<cdot>(dq2, to_ag (Some v2))])))" by (metis map_op op_heap.simps)
+  from upred_entails_wand_holdsR2[OF upred_entail_eqL[OF discrete_valid] this] 
+  have "upred_f_holds ((l \<mapsto>{dq1} v1) -\<^emph> (l \<mapsto>{dq2} v2) -\<^emph> 
+    \<upharpoonleft>(All (heap_rel [l\<mapsto>(dq1\<cdot>dq2, to_ag (Some v1)\<cdot>to_ag (Some v2))])))" 
+    by (auto simp: valid_raw_heap.rep_eq valid_def op_prod_def)
+  then have "upred_f_holds ((l \<mapsto>{dq1} v1) -\<^emph> (l \<mapsto>{dq2} v2) -\<^emph> 
+    \<upharpoonleft>(valid (dq1\<cdot>dq2) \<and> (\<forall>n. \<exists>ag. n_equiv n (to_ag (Some v1)\<cdot>to_ag (Some v2)) (to_ag ag))))"
+    by (smt (verit, ccfv_threshold) camera_comm camera_valid_op dcamera_valid_iff fun_upd_same 
+      points_to_valid upred_entails_wand_holdsR upred_holds_entails)
+  then have "upred_f_holds ((l \<mapsto>{dq1} v1) -\<^emph> (l \<mapsto>{dq2} v2) -\<^emph> 
+    \<upharpoonleft>(\<forall>n. \<exists>ag. n_equiv n (to_ag (Some v1)\<cdot>to_ag (Some v2)) (to_ag ag)))"
+    using upred_entails_wand_holdsR2 pure_entailsI by (metis (no_types, lifting))
+  then have "upred_f_holds ((l \<mapsto>{dq1} v1) -\<^emph> (l \<mapsto>{dq2} v2) -\<^emph> 
+    \<upharpoonleft>(\<exists>ag. to_ag (Some v1)\<cdot>to_ag (Some v2) = to_ag ag))" using d_equiv by (smt (verit, ccfv_SIG))
+  then show ?thesis 
+    by (smt (z3) option.inject pure_entailsI singleton_inject to_ag.rep_eq to_ag_op upred_entails_wand_holdsR2)
+qed
 end
